lemma_map_is_distinct 증명 성공! 만세!

src/common/Nemonuri.IndexMap.Unique.fst
@@ -90,23 +90,33 @@ let map_is_distinct (#data_t:eqtype) (map:t data_t)
   forall (x2:key_t map{x2 < x1}). 
     ~(equal_selection_key map x1 x2)
 
-//let map_is_distinct
 
-
-let lemma_is_distinct (#data_t:eqtype) (m:t data_t)
+let lemma_map_is_distinct (#data_t:eqtype) (m:t data_t)
   : Lemma ((map_is_distinct m) <==> (forall (x:key_t m). (unique_key_predicate m x)))
   =
   let pl = (map_is_distinct m) in
   let pr = (forall (x:key_t m). (unique_key_predicate m x)) in
   let pr1 = (forall (x:key_t m). (Lu.predicate_is_linear_unique 0 (count m) (equal_selection_key m x) x)) in
   let pl1 = (forall (x1 x2:key_t m). (x1 <> x2) ==> ~(equal_selection_key m x1 x2)) in
-
-  let lemma_pr_pr1' () : Lemma (pr <==> pr1) =
+  let lemma_pr_ep_pr1' () : Lemma (pr <==> pr1) =
     Cl.forall_intro (lemma_unique_key_predicate m)
   in
-  let lemma_pl_pl1' () : Lemma (pl <==> pl1) =
-    admit ()
+  let lemma_pl_ep_pl1' () : Lemma (pl <==> pl1) =
+    (* Note: 이건 당연히 쉽게 증명 될 것이다. *)
+    assert (pl1 ==> pl);
+    let lemma_pl_to_pl1' () : Lemma (requires pl) (ensures pl1) =
+      (* Note: 
+         - 이런 꼴의 증명 방식, 나중에 많이 쓰일 것 같은데.
+         - 필요할 때 일반화 해야지. *)
+      let lemma_pl_to_pl1'' (x1 x2:key_t m) 
+        : Lemma (requires x1 <> x2) (ensures ~(equal_selection_key m x1 x2)) =
+        match x1 < x2 with
+        | true -> assert (~(equal_selection_key m x2 x1))
+        | false -> assert (~(equal_selection_key m x1 x2))
+      in
+      Cl.move_requires_2 lemma_pl_to_pl1'' |> Cl.forall_intro_2
+    in
+    Cl.move_requires lemma_pl_to_pl1' ()
   in
-
-  lemma_pr_pr1' ();
-  lemma_pl_pl1' ()
+  lemma_pr_ep_pr1' ();
+  lemma_pl_ep_pl1' ()
